We start from the expression for the
hydrogen potential in position basis.
TODO-Derive??
\begin{equation}
    V(\vec{r}) = \frac{e^2}{4 \pi \epsilon_0}(
    -\frac{1}{r}
    + \pi a_0^3\int{\frac{e^{-\frac{2r}{a_0}}}{
            \abs{\vec{r} - \vec{r'}}} d\vec{r}'})
\end{equation}
using two standard results
\begin{eqnarray}
    \int{\frac{1}{r} e^{i\vec{q}.\vec{r}} d^3\vec{r}}
    &=& \frac{4 \pi}{q^2}\\
    \int{e^{-\alpha r} e^{i\vec{q}.\vec{r}} d^3\vec{r}}
    &=& \frac{8 \pi \alpha}{{(\alpha^2 + q^2)}^2}\\
\end{eqnarray}
with \(\alpha = \frac{2}{a_0}\) we end up
with
\begin{eqnarray}
    V(\vec{q}) &=& \frac{e^2}{4 \pi \epsilon_0}(
    - \frac{4\pi}{q^2}
    + \frac{\pi a_0^3}{q^2}
    \frac{8 \pi \alpha}{{(\alpha^2 + q^2)}^2})\\
    &=& \frac{e^2}{\epsilon_0 q^2}(
    \frac{ \alpha^4}{{(\alpha^2 + q^2)}^2} - 1
    )
\end{eqnarray}